Examples/UniswapV2Pair/Correct.lean
@@ -1,19 +1,29 @@
 import Examples.UniswapV2Pair.Bytecode
+import Examples.UniswapV2Pair.Dispatch
 import Examples.UniswapV2Pair.Allowance
+import Examples.UniswapV2Pair.Approve
 import Examples.UniswapV2Pair.BalanceOf
 import Examples.UniswapV2Pair.Decimals
 import Examples.UniswapV2Pair.DomainSeparator
 import Examples.UniswapV2Pair.Factory
 import Examples.UniswapV2Pair.GetReserves
+import Examples.UniswapV2Pair.Initialize
 import Examples.UniswapV2Pair.KLast
 import Examples.UniswapV2Pair.MinimumLiquidity
 import Examples.UniswapV2Pair.Nonces
 import Examples.UniswapV2Pair.PermitTypehash
 import Examples.UniswapV2Pair.Price0CumulativeLast
 import Examples.UniswapV2Pair.Price1CumulativeLast
+import Examples.UniswapV2Pair.Skim
+import Examples.UniswapV2Pair.Sync
 import Examples.UniswapV2Pair.Token0
 import Examples.UniswapV2Pair.Token1
 import Examples.UniswapV2Pair.TotalSupply
+import Examples.UniswapV2Pair.Transfer
+import Examples.UniswapV2Pair.TransferFrom
+import Examples.UniswapV2Pair.TransferFromFinite
+import Examples.UniswapV2Pair.TransferFromSuccess
+import Examples.UniswapV2Pair.TransferFromDecode
 import Solm.Equiv
 
 /-!
