Solm.lean
@@ -1,4 +1,5 @@
 import Solm.Syntax
+import Solm.Notation
 import Solm.Value
 import Solm.Storage
 import Solm.Semantics
